src/exchange_proof.v
@@ -1,0 +1,197 @@
+From iris.algebra Require Export cmra.
+From iris.algebra Require Import proofmode_classes.
+From iris.prelude Require Import options.
+Require Import Burrow.CpdtTactics.
+
+From stdpp Require Import gmap.
+From stdpp Require Import mapset.
+From stdpp Require Import sets.
+From stdpp Require Import list.
+Require Import Burrow.gmap_utils.
+Require Import Burrow.rollup.
+Require Import Burrow.indexing.
+Require Import Burrow.locations.
+
+Require Import coq_tricks.Deex.
+
+Context {M} `{!EqDecision M} `{!Countable M} `{!TPCM M}.
+Context {RI} `{!EqDecision RI, !Countable RI, !RefinementIndex M RI}.
+
+Definition specific_exchange_cond (ref: Refinement M M) (p m f h s m' f' h' s' : M) :=
+  ∃ j mh ,
+  match rel M M ref (dot f p) with
+  | None => True
+  | Some i1 => m_valid (dot m i1) ->
+      dot j s' = f' /\ m' = dot h' mh /\
+      match rel M M ref (dot (dot j s) p) with
+      | None => False
+      | Some i2 => mov (dot m i1) (dot (dot h mh) i2)
+      end
+  end.
+
+Definition specific_flow_cond p i (t t': Branch M) (active: Lifetime) (down up : PathLoc -> M) :=
+  let q := (p, i) in
+  let r := (p, S i) in
+  let s := (p ++ [i], 0) in
+  specific_exchange_cond (refinement_of_nat M RI i)
+      (node_total_minus_live (refinement_of_nat M RI) (node_of_pl t q) active)
+      (down q) (node_live (node_of_pl t q))
+      (down r) (down s)
+      (up q) (node_live (node_of_pl t' q))
+      (up r) (up s).
+
+Lemma branchcons_pl t p i
+  : branch_of_pl t (p, i) ≡ BranchCons (node_of_pl t (p, i)) (branch_of_pl t (p, S i)).
+  Admitted.
+  
+Lemma cellnode_pl t p i
+  : node_of_pl t (p, i) ≡ CellNode (cell_of_pl t (p, i)) (branch_of_pl t (p++[i], 0)).
+  Admitted.
+  
+Lemma branchcons_pl_inv_b t p i b n
+  : branch_of_pl t (p, i) ≡ BranchCons n b ->
+      b ≡ branch_of_pl t (p, S i).
+  Admitted.
+  
+Lemma branchcons_pl_inv_n t p i b n
+  : branch_of_pl t (p, i) ≡ BranchCons n b ->
+      n ≡ node_of_pl t (p, i).
+  Admitted.
+
+Definition branch_of_node (node: Node M) := match node with CellNode _ b => b end.
+
+Lemma branch_of_node_node_of_pl t p i
+  : branch_of_node (node_of_pl t (p, i)) ≡ branch_of_pl t (p++[i], 0). Admitted.
+
+Global Instance branch_of_node_proper :
+  Proper ((≡) ==> (≡)) branch_of_node. Admitted.
+
+Lemma cell_total_split (cell: Cell M) lt :
+  cell_total cell lt = dot (cell_live cell) (cell_total_minus_live cell lt). Admitted.
+  
+Tactic Notation "full_generalize" constr(t) "as" simple_intropattern(name) :=
+  let EQ := fresh in
+  let name1 := fresh in
+  assert (exists x , x = t) as EQ by (exists t; trivial); destruct EQ as [name1];
+    try (rewrite <- EQ);
+    (repeat match reverse goal with  
+    | [H : context[t] |- _ ] => rewrite <- EQ in H
+    end); clear EQ; try (clear name); rename name1 into name.
+    
+Lemma all_the_movs (z m f h s r k m' f' h' s' r' k' : M) i
+  (mo: mov (dot r s) (dot r' s'))
+  (inr: in_refinement_domain (refinement_of_nat M RI) i (dot f (dot z r)))
+  (myflow : specific_exchange_cond (refinement_of_nat M RI i) (dot z r) m f h s m' f' h' s')
+  (val : m_valid (dot m (project (refinement_of_nat M RI) i (dot (dot f z) r))))
+  : mov (dot (dot (project (refinement_of_nat M RI) i (dot (dot f z) r)) k) m)
+    (dot (dot (project (refinement_of_nat M RI) i (dot (dot f' z) r')) k') m').
+Proof.
+  unfold specific_exchange_cond in myflow. deex.
+  unfold in_refinement_domain in inr.
+  unfold project in *.
+  replace ((dot (dot f z) r)) with (dot f (dot z r)) in val
+    by (apply tpcm_assoc).
+  destruct (rel M M (refinement_of_nat M RI i) (dot f (dot z r))).
+  - rename m0 into a.
+    have myf := myflow val. clear myflow.
+    destruct_ands.
+    
+  
+
+
+Lemma specexc_branch t t' active (branch branch': Branch M) p i
+  (down up : PathLoc -> M)
+  (flow_update : ∀ p i , specific_flow_cond p i t t' active down up)
+  (branch_is : branch ≡ branch_of_pl t (p, i))
+  (branch'_is : branch' ≡ branch_of_pl t' (p, i))
+  (batird : branch_all_total_in_refinement_domain (refinement_of_nat M RI) branch active i)
+          : branch_all_total_in_refinement_domain (refinement_of_nat M RI) branch' active i
+      /\ mov
+        (dot (branch_total (refinement_of_nat M RI) branch active i) (down (p, i)))
+        (dot (branch_total (refinement_of_nat M RI) branch' active i) (up (p, i)))
+with specexc_node t t' active (node node': Node M) p i
+  (down up : PathLoc -> M)
+  (flow_update : ∀ p i , specific_flow_cond p i t t' active down up)
+  (node_is : node ≡ node_of_pl t (p, i))
+  (node'_is : node' ≡ node_of_pl t' (p, i))
+  (batird : node_all_total_in_refinement_domain (refinement_of_nat M RI) node active i)
+          : node_all_total_in_refinement_domain (refinement_of_nat M RI) node' active i
+      /\ mov
+        (dot (branch_total (refinement_of_nat M RI) (branch_of_node node) active 0) (down (p++[i], 0)))
+        (dot (branch_total (refinement_of_nat M RI) (branch_of_node node') active 0) (up (p++[i], 0))).
+Proof.
+ - destruct branch'.
+   + rename n into n'.
+     have branch_destruct := branchcons_pl t p i.
+     have triv_equiv : (branch_of_pl t (p, S i) ≡ branch_of_pl t (p, S i)) by trivial.
+     have triv_equiv2 : (node_of_pl t (p, i) ≡ node_of_pl t (p, i)) by trivial.
+     have b_equiv : branch' ≡ branch_of_pl t' (p, S i)
+        by (apply branchcons_pl_inv_b with (n := n'); symmetry; trivial).
+     have n_equiv : n' ≡ node_of_pl t' (p, i)
+        by (apply branchcons_pl_inv_n with (b := branch'); symmetry; trivial).
+     have IHbranch := specexc_branch t t' active (branch_of_pl t (p, S i)) branch' p (S i)
+                          down up flow_update triv_equiv b_equiv.
+     clear specexc_branch.
+     have IHnode := specexc_node t t' active (node_of_pl t (p, i)) n' p i
+                          down up flow_update triv_equiv2 n_equiv.
+     clear specexc_node.
+     
+     setoid_rewrite branch_is in batird.
+     setoid_rewrite branch_destruct in batird.
+     rewrite branch_all_total_in_refinement_domain_unfold in batird.
+     destruct_ands.
+     
+     have IHbranch' := IHbranch H0. clear IHbranch.
+     have IHnode' := IHnode H. clear IHnode.
+        destruct_ands.
+     split.
+     * unfold branch_all_total_in_refinement_domain. split; trivial.
+     * setoid_rewrite branch_is. setoid_rewrite branch_destruct.
+        rewrite branch_total_unfold.
+        have myflow := flow_update p i.
+        unfold specific_flow_cond in myflow.
+        setoid_rewrite cellnode_pl.
+        setoid_rewrite cellnode_pl in myflow.
+        unfold node_total_minus_live in myflow.
+        rewrite (branch_total_unfold (refinement_of_nat M RI) (BranchCons n' branch')).
+        setoid_rewrite n_equiv.
+        rewrite node_total_unfold.
+        setoid_rewrite (cellnode_pl t' p i).
+        rewrite node_total_unfold.
+        setoid_rewrite b_equiv.
+        setoid_rewrite branch_of_node_node_of_pl in H2.
+        setoid_rewrite n_equiv in H2.
+        setoid_rewrite branch_of_node_node_of_pl in H2.
+        unfold node_live in myflow.
+        rewrite cell_total_split.
+        rewrite cell_total_split.
+        setoid_rewrite b_equiv in H4.
+        full_generalize
+          (branch_total (refinement_of_nat M RI) (branch_of_pl t (p, S i)) active (S i))
+          as k.
+        full_generalize
+          (branch_total (refinement_of_nat M RI) (branch_of_pl t' (p, S i)) active (S i))
+          as k'.
+        full_generalize (cell_live (cell_of_pl t (p, i))) as f.
+        full_generalize (cell_live (cell_of_pl t' (p, i))) as f'.
+        full_generalize (cell_total_minus_live (cell_of_pl t (p, i)) active) as z.
+        full_generalize (cell_total_minus_live (cell_of_pl t' (p, i)) active) as z'.
+        full_generalize (branch_total (refinement_of_nat M RI) (branch_of_pl t (p ++ [i], 0)) active 0) as r.
+        full_generalize (branch_total (refinement_of_nat M RI) (branch_of_pl t' (p ++ [i], 0)) active 0) as r'.
+        full_generalize (down (p, S i)) as h.
+        full_generalize (up (p, S i)) as h'.
+        full_generalize (down (p, i)) as m.
+        full_generalize (up (p, i)) as m'.
+        full_generalize ((down (p ++ [i], 0))) as s.
+        full_generalize ((up(p ++ [i], 0))) as s'.
+        unfold specific_exchange_cond in myflow.
+
+ 
+Lemma specific_flows_preserve_branch_all_total_in_refinement_domain t t' active
+  (down up : PathLoc -> M)
+  (flow_update : ∀ p i , specific_flow_cond p i t t' active down up)
+  (down_0 : down ([], 0) = unit)
+  (up_0 : up ([], 0) = unit)
+  (batird : branch_all_total_in_refinement_domain (refinement_of_nat M RI) t active 0)
+          : branch_all_total_in_refinement_domain (refinement_of_nat M RI) t' active 0.
+Proof.
